FreydSSA.lean
@@ -7,11 +7,11 @@ import FreydSSA.Terminator.Extrinsic.Subst
 import FreydSSA.BasicBlock.Extrinsic.Basic
 import FreydSSA.BasicBlock.Extrinsic.Subst
 import FreydSSA.CFG.Extrinsic.Basic
--- import FreydSSA.CFG.Extrinsic.Subst
+import FreydSSA.CFG.Extrinsic.Subst
 import FreydSSA.Region.Extrinsic.Basic
--- import FreydSSA.Region.Extrinsic.Subst
+import FreydSSA.Region.Extrinsic.Subst
 import FreydSSA.GRegion.Extrinsic.Basic
--- import FreydSSA.GRegion.Extrinsic.Subst
+import FreydSSA.GRegion.Extrinsic.Subst
 import FreydSSA.Term.Intrinsic.Basic
 import FreydSSA.Term.Intrinsic.Subst
 import FreydSSA.Body.Intrinsic.Basic
@@ -27,7 +27,21 @@ import FreydSSA.Region.Intrinsic.Basic
 import FreydSSA.GRegion.Intrinsic.Basic
 -- import FreydSSA.GRegion.Intrinsic.Subst
 
--- TODO: Intrinsic BodyM, Body' ==> fix Intrinsic BB
+import FreydSSA.Term.Fun.Basic
+-- import FreydSSA.Term.Fun.Subst
+-- import FreydSSA.Body.Fun.Basic
+-- import FreydSSA.Body.Fun.Subst
+-- import FreydSSA.Terminator.Fun.Basic
+-- import FreydSSA.Terminator.Fun.Subst
+-- import FreydSSA.BasicBlock.Fun.Basic
+-- import FreydSSA.BasicBlock.Fun.Subst
+-- import FreydSSA.CFG.Fun.Basic
+-- import FreydSSA.CFG.Fun.Subst
+-- import FreydSSA.Region.Fun.Basic
+-- import FreydSSA.Region.Fun.Subst
+-- import FreydSSA.GRegion.Fun.Basic
+-- import FreydSSA.GRegion.Fun.Subst
+
 -- TODO: Indexed intrinsic/extrinsic (dominator tree)
 -- TODO: Dominated intrinsic/extrinsic (dominator tree)
 -- TODO: capture-avoiding subst over extrinsic (which is just Γ ⊢ b ▷ Γ for blocks!)
@@ -43,4 +57,3 @@ import FreydSSA.GRegion.Intrinsic.Basic
   -- TODO: use dominator quotient?
 -- TODO: Initial model for Elgot: show quotient respects Elgot rules
   -- TODO: use dominator quotient?
--- TODO: try contexts as (partial) functions?
