FreydSSA/Term/Fun/Basic.lean
@@ -1,0 +1,80 @@
+import Mathlib.Logic.Lemmas
+
+import FreydSSA.Ctx.Var.Fun
+import FreydSSA.InstSet
+import FreydSSA.Untyped
+
+variable {φ ν α} [Φ : InstSet φ (Ty α)]
+  [Φc : CohInstSet φ (Ty α)]
+  [DecidableEq ν] [DecidableEq α]
+
+inductive UTm.FWf : Purity → FCtx ν (Ty α) → UTm φ ν → Ty α → Type _
+  | var (p) {A : Ty α} : Γ x = (A : WithBot _) → FWf p Γ (var x) A
+  | op : Φ.Op f p A B → FWf 1 Γ e A → FWf p Γ (op f e) B
+  | pair (p) : FWf 1 Γ l A → FWf 1 Γ r B → FWf p Γ (pair l r) (A.pair B)
+  | unit (p) : FWf p Γ unit Ty.unit
+  | bool (p b) : FWf p Γ (bool b) Ty.bool
+
+variable {Γ Δ : FCtx ν (Ty α)}
+
+def UTm.FWf.of_pure {e : UTm φ ν} : e.FWf 1 Γ A → e.FWf p Γ A
+  | var _ w => var p w
+  | op hf de => op hf.of_pure (de.of_pure)
+  | pair _ dl dr => pair p (dl.of_pure) (dr.of_pure)
+  | unit _ => unit p
+  | bool _ b => bool p b
+
+theorem FCtx.Cmp.tyEq {Γ Δ : FCtx ν (Ty α)} {e : UTm φ ν}
+  (c : Γ.Cmp Δ) (de : UTm.FWf p Γ e A) (de' : UTm.FWf p' Δ e A') : A = A'
+  := by induction de generalizing p' Δ A' with
+  | var _ w => cases de' with | var _ w' => exact c.var_eq _ _ _ w w'
+  | op hf _ I => cases de' with | op hf' de' => exact Φc.coh_trg' hf hf' (I c de')
+  | pair _ _ _ I1 I2 => cases de' with | pair _ dl' dr' => rw [I1 c dl', I2 c dr']
+  | _ => cases de'; rfl
+
+theorem UTm.FWf.tyEq {e : UTm φ ν} (de : e.FWf p Γ A) (de' : e.FWf p' Γ A')
+  : A = A' := (FCtx.Cmp.refl Γ).tyEq de de'
+
+theorem UTm.FWf.allEq {e : UTm φ ν}
+  (de : e.FWf p Γ A) (de' : e.FWf p Γ A) : de = de' := by induction de with
+  | var _ w => cases de' with | var _ w' => rfl
+  | op hf de I => cases de' with | op hf' de' =>
+    cases de.tyEq de'
+    rw [I de']
+  | pair _ dl dr Il Ir => cases de' with | pair _ dl' dr' => rw [Il dl', Ir dr']
+  | _ => cases de'; rfl
+
+theorem UTm.FWf.allHeq {e : UTm φ ν}
+  (de : e.FWf p Γ A) (de' : e.FWf p Γ A') : HEq de de'
+  := by cases de.tyEq de'; apply Eq.heq; apply allEq
+
+def UTm.FWf.wk {e : UTm φ ν} (w : Γ.Wk Δ) : e.FWf p Δ A → e.FWf p Γ A
+  | var p w' => var p (w.var _ _ w')
+  | op hf de => op hf (de.wk w)
+  | pair p dl dr => pair p (dl.wk w) (dr.wk w)
+  | unit p => unit p
+  | bool p b => bool p b
+
+def UTm.FWf.linf {e : UTm φ ν} : e.FWf p Γ A → e.FWf p' Δ A' → e.FWf p (Γ.linf Δ) A
+  | var p w, var _ w' => var p (by rw [FCtx.linf_right_var_eq_left _ _ w']; exact w)
+  | op hf de, op _ de' => op hf (de.linf de')
+  | pair p dl dr, pair _ dl' dr' => pair p (dl.linf dl') (dr.linf dr')
+  | unit p, _ => unit p
+  | bool p b, _ => bool p b
+
+def UTm.FWf.rinf {e : UTm φ ν} : e.FWf p Γ A → e.FWf p' Δ A' → e.FWf p' (Γ.rinf Δ) A'
+  | var _ w, var p' w' => var p' (by rw [FCtx.rinf_left_var_eq_right _ _ w]; exact w')
+  | op _ de, op hf' de' => op hf' (de.rinf de')
+  | pair _ dl dr, pair p' dl' dr' => pair p' (dl.rinf dl') (dr.rinf dr')
+  | _, unit p' => unit p'
+  | _, bool p' b => bool p' b
+
+def FCtx.Cmp.wfInf {e : UTm φ ν} (c : Γ.Cmp Δ) : e.FWf p Γ A → e.FWf p' Δ A' → e.FWf p (Γ.inf Δ) A
+  | UTm.FWf.var p w, UTm.FWf.var _ w' => UTm.FWf.var p
+    (by rw [c.inf_eq_linf, linf_right_var_eq_left _ _ w']; exact w)
+  | UTm.FWf.op hf de, UTm.FWf.op _ de' => UTm.FWf.op hf (c.wfInf de de')
+  | UTm.FWf.pair p dl dr, UTm.FWf.pair _ dl' dr' => UTm.FWf.pair p (c.wfInf dl dl') (c.wfInf dr dr')
+  | UTm.FWf.unit p, _ => UTm.FWf.unit p
+  | UTm.FWf.bool p b, _ => UTm.FWf.bool p b
+
+--TODO: cmp ==> inf = linf without alleq, rinf with
